common/BlockNames.v
@@ -1,0 +1,147 @@
+Require Import Coqlib.
+Require Import AST.
+Require Import Maps.
+
+(** * Interfaces *)
+
+Module Type BlockType <: EQUALITY_TYPE.
+  Parameter t : Type.
+  Parameter eq : forall b1 b2 : t, {b1 = b2} + {b1 <> b2}.
+
+  Parameter glob : ident -> t.  (* block associated to a global identifier *)
+  Parameter init : t.           (* initial dynamic block id *)
+  Parameter succ : t -> t.
+
+  Parameter lt : t -> t -> Prop.
+  Parameter lt_dec : forall b1 b2, {lt b1 b2} + {~ lt b1 b2}.
+
+  Axiom lt_glob_init : forall i, lt (glob i) init.
+  Axiom lt_succ : forall b, lt b (succ b).
+  Axiom lt_trans : forall x y z, lt x y -> lt y z -> lt x z.
+  Axiom lt_strict : forall b, ~ lt b b.
+  Axiom lt_succ_inv: forall x y, lt x (succ y) -> lt x y \/ x = y.
+End BlockType.
+
+Module Type BMapType (M: BlockType).
+  Definition elt := M.t.
+  Definition elt_eq := M.eq.
+  Parameter t: Type -> Type.
+  Parameter init: forall {A}, A -> t A.
+  Parameter get: forall {A}, elt -> t A -> A.
+  Parameter set: forall {A}, elt -> A -> t A -> t A.
+  Axiom gi: forall {A} i (x: A), get i (init x) = x.
+  Axiom gss: forall {A} i (x: A) m, get i (set i x m) = x.
+  Axiom gso: forall {A} i j (x: A) m, i <> j -> get i (set j x m) = get i m.
+  Axiom gsspec:
+    forall {A} i j (x: A) m, get i (set j x m) = (if elt_eq i j then x else get i m).
+  Axiom gsident:
+    forall {A} i j (m: t A), get j (set i (get i m) m) = get j m.
+  Parameter map: forall {A B}, (A -> B) -> t A -> t B.
+  Axiom gmap:
+    forall {A B} (f: A -> B) i m, get i (map f m) = f (get i m).
+  Axiom set2:
+    forall {A} i (x y: A) m, set i y (set i x m) = set i y m.
+End BMapType.
+
+(** * Implementation *)
+
+Module Block : BlockType.
+  Inductive t_def :=
+    | glob_def : ident -> t_def
+    | dyn : positive -> t_def.
+
+  Definition t := t_def.
+
+  Definition eq (b1 b2 : t):
+    {b1 = b2} + {b1 <> b2}.
+  Proof.
+    decide equality.
+    apply peq.
+    apply peq.
+  Defined.
+
+  Definition glob := glob_def.
+  Definition init := dyn 1%positive.
+
+  Definition succ (b: t) :=
+    match b with
+      | glob_def i => glob (Pos.succ i)
+      | dyn n => dyn (Pos.succ n)
+    end.
+
+  Inductive lt_def : t -> t -> Prop :=
+    | glob_dyn_lt i n:
+        lt_def (glob i) (dyn n)
+    | glob_lt m n:
+        Pos.lt m n ->
+        lt_def (glob m) (glob n)
+    | dyn_lt m n:
+        Pos.lt m n ->
+        lt_def (dyn m) (dyn n).
+
+  Definition lt := lt_def.
+
+  Definition lt_dec b1 b2:
+    {lt b1 b2} + {~ lt b1 b2}.
+  Proof.
+    destruct b1 as [i1|n1], b2 as [i2|n2].
+    - destruct (plt i1 i2).
+      + left. abstract (constructor; eauto).
+      + right. abstract (inversion 1; eauto).
+    - left. abstract constructor.
+    - right. abstract (inversion 1).
+    - destruct (plt n1 n2).
+      + left. abstract (constructor; eauto).
+      + right. abstract (inversion 1; eauto).
+  Defined.
+
+  Lemma lt_glob_init i:
+    lt (glob i) init.
+  Proof.
+    constructor.
+  Qed.
+
+  Lemma lt_succ b:
+    lt b (succ b).
+  Proof.
+    destruct b; constructor; xomega.
+  Qed.
+
+  Lemma lt_trans x y z:
+    lt x y -> lt y z -> lt x z.
+  Proof.
+    intros Hxy Hyz.
+    destruct Hyz; inv Hxy; constructor; xomega.
+  Qed.
+
+  Lemma lt_strict b:
+    ~ lt b b.
+  Proof.
+    inversion 1; eapply Plt_strict; eauto.
+  Qed.
+
+  Lemma lt_succ_inv x y:
+    lt x (succ y) -> lt x y \/ x = y.
+  Proof.
+    destruct y; simpl; inversion 1; subst.
+    - destruct (Plt_succ_inv m i) as [H1|H1]; auto.
+      left; constructor; auto.
+      right; subst; reflexivity.
+    - left; constructor.
+    - destruct (Plt_succ_inv m p) as [H1|H1]; auto.
+      left; constructor; auto.
+      right; subst; reflexivity.
+  Qed.
+End Block.
+
+Module BMap : BMapType Block := EMap Block.
+
+(** * Properties *)
+
+Lemma Blt_trans_succ b1 b2:
+  Block.lt b1 b2 -> Block.lt b1 (Block.succ b2).
+Proof.
+  intros H.
+  eapply Block.lt_trans; eauto.
+  apply Block.lt_succ.
+Qed.
